Separated EO code and models; make EO models transparent in main proof

fairis/heap_lang/examples/even_odd/interface.v
@@ -13,37 +13,6 @@ Proof.
   intros [x] [y]. destruct (decide (x = y)); [left | right]; set_solver.
 Qed. 
 
-Class threadG Σ := ThreadG {
-  th_name: gname;
-  th_n_G :> inG Σ (excl_authR natO);
-}.
-
-Class threadPreG Σ := {
-  thread_PreG :> inG Σ (excl_authR natO);
-}.
-
-Section ThreadGLemmas.
-  Context `{!threadG Σ}.
-
-  Definition th_at (n: nat) := own th_name (◯E n).
-  Definition auth_th_at (n: nat) := own th_name (●E n).
-  
-  Lemma th_agree γ (N M: nat) :
-    own γ (◯E N) -∗ own γ (●E M) -∗ ⌜ M = N ⌝.
-  Proof.
-    iIntros "HA HB". iCombine "HB HA" as "H".
-    iDestruct (own_valid with "H") as "%Hval".
-    iPureIntro. by apply excl_auth_agree_L.
-  Qed.
-  
-  Lemma th_update γ (N M P: nat) :
-    own γ (●E N) ∗ own γ (◯E M) ==∗ own γ (●E P) ∗ own γ (◯E P).
-  Proof.
-    rewrite -!own_op. iApply own_update. apply excl_auth_update.
-  Qed.
-
-End ThreadGLemmas.
-
 Definition BuildSubModel (St Priv Role: Type) Trans := {|
    amSt := St;
    amA := PubA + Priv;
@@ -86,62 +55,7 @@ Record EvenModel := {
       (STEP: amTrans even_AM st__e (inl (step_sync M), None) st__e'):
       AM_live_roles ame_strong st__e' ⊆ AM_live_roles ame_strong st__e;
 
-  even_corr 
-    {M__p : FairModel} {LM__p : LiveModel heap_lang M__p}
-    {Σ : gFunctors} {heapGS0 : heapGS Σ LM__p}
-    (threadG0 : threadG Σ) 
-  (proj_st : M__p → amSt even_AM) (l : loc) (st : M__p) 
-  (N : nat) :=
-  (* let st__t := proj_st st in *)
-  (frag_model_is st ∗ l ↦ #N ∗ (* ⌜cur_even st__t N⌝ ∗ *)
-   own th_name (●E (if Nat.even N then N else N + 1)))%I;
-  (* glob_step_even {M__p : FairModel} *)
-  (*   (proj_st : fmstate M__p → amSt even_AM) *)
-  (* (lift_role : amRole even_AM → fmrole M__p)  *)
-  (* (st st' : M__p) (ρ__t : amRole even_AM) (st__e' : amSt even_AM) :=  *)
-  (* proj_st st' = st__e' *)
-  (* ∧ fmtrans M__p st (Some (lift_role ρ__t)) st' *)
-  (*   ∧ (AM_live_roles ame_strong (proj_st st') *)
-  (*      ⊆ AM_live_roles ame_strong (proj_st st) *)
-  (*      → live_roles M__p st' ⊆ live_roles M__p st); *)
-  even_vs {M__p : FairModel} {LM__p : LiveModel heap_lang M__p} 
-  {Σ : gFunctors} {heapGS0 : heapGS Σ LM__p} {threadG0 : threadG Σ} 
-  (proj_st : fmstate M__p → amSt even_AM) (lift_role : 
-                                            amRole even_AM → 
-                                            fmrole M__p) 
-  (l : loc) (ι : namespace) (ρ__t : amRole even_AM) tid := 
-  (□ (|={⊤,⊤ ∖ ↑ι}=>
-        ∃ (st__p : M__p) (N : nat),
-          let st__t := proj_st st__p in
-          ▷ even_corr threadG0 proj_st l st__p N ∗
-          (∀ f, tid ↦M {[ lift_role ρ__t := f ]} -∗ frag_model_is st__p -∗ frag_free_roles_are ∅ -∗
-             MU (⊤ ∖ ↑ι) tid (
-               ∃ st__p' f', tid ↦M {[ lift_role ρ__t := f' ]}  ∗ frag_model_is st__p' ∗ frag_free_roles_are ∅ ∗ ⌜ f' > 43 ⌝ ∗
-                 (▷ (even_corr threadG0 proj_st l st__p' (if Nat.even N then N + 1 else N)) ={⊤ ∖ ↑ι, ⊤}=∗ True)))
-          ))%I;
-          (* ∗ *)
-
-          (* (⌜Nat.odd N⌝ *)
-          (*  → ∀ (st__t' : amSt even_AM) (a : ePriv), *)
-          (*      ⌜amTrans even_AM st__t (inr a, Some ρ__t) st__t'⌝ ∗ *)
-          (*      ⌜cur_even st__t' N⌝ *)
-          (*      → ∃ st__p' : M__p, *)
-          (*          ⌜glob_step_even proj_st lift_role st__p st__p' ρ__t st__t'⌝ ∗ *)
-          (*          (▷ even_corr threadG0 proj_st l st__p' N ={⊤ ∖ ↑ι,⊤}=∗ True))))%I; *)
-  even_prog: val;
-  even_spec {M__p : FairModel} {LM__p : LiveModel heap_lang M__p} 
-  {Σ : gFunctors} {heapGS0 : heapGS Σ LM__p} {threadG0 : threadG Σ} 
-  (proj_st : M__p → amSt even_AM) (lift_role: amRole even_AM → fmrole M__p) 
-  (tid : locale heap_lang) (n : loc) (ρ__t : amRole even_AM) 
-  (N f : nat) (FUEL: f > 40) (ι : namespace) (FL: ∀ st : M__p, lm_fl LM__p st ≥ 61):
-      {{{ even_vs proj_st lift_role n ι ρ__t tid ∗
-        tid ↦M {[lift_role ρ__t := f]} ∗
-        own th_name (◯E N) ∗
-        frag_free_roles_are ∅ }}}
-          even_prog #n #N@tid
-        {{{ RET #(); tid ↦M ∅ }}};
-
-  ρ__e: amRole even_AM;
+    ρ__e: amRole even_AM;
 }.
 
 
@@ -168,61 +82,5 @@ Record OddModel := {
       (STEP: amTrans odd_AM st__e (inl (step_sync M), None) st__e'):
       AM_live_roles ame_strong st__e' ⊆ AM_live_roles ame_strong st__e;
 
-  odd_corr 
-    {M__p : FairModel} {LM__p : LiveModel heap_lang M__p}
-    {Σ : gFunctors} {heapGS0 : heapGS Σ LM__p}
-    (threadG0 : threadG Σ) 
-  (proj_st : M__p → amSt odd_AM) (l : loc) (st : M__p) 
-  (N : nat) :=
-  let st__t := proj_st st in
-  (frag_model_is st ∗ l ↦ #N ∗ ⌜cur_odd st__t N⌝ ∗
-   own th_name (●E (if Nat.odd N then N else N + 1)))%I;
-  glob_step_odd {M__p : FairModel}
-    (proj_st : fmstate M__p → amSt odd_AM)
-  (lift_role : amRole odd_AM → fmrole M__p) 
-  (st st' : M__p) (ρ__t : amRole odd_AM) (st__e' : amSt odd_AM) := 
-  proj_st st' = st__e'
-  ∧ fmtrans M__p st (Some (lift_role ρ__t)) st'
-    ∧ (AM_live_roles ame_strong (proj_st st')
-       ⊆ AM_live_roles ame_strong (proj_st st)
-       → live_roles M__p st' ⊆ live_roles M__p st);
-  odd_vs {M__p : FairModel} {LM__p : LiveModel heap_lang M__p} 
-  {Σ : gFunctors} {heapGS0 : heapGS Σ LM__p} {threadG0 : threadG Σ} 
-  (proj_st : fmstate M__p → amSt odd_AM) (lift_role : 
-                                            amRole odd_AM → 
-                                            fmrole M__p) 
-  (l : loc) (ι : namespace) (ρ__t : amRole odd_AM) := 
-  (□ (|={⊤,⊤ ∖ ↑ι}=>
-        ∃ (st__p : M__p) (N : nat),
-          let st__t := proj_st st__p in
-          ▷ odd_corr threadG0 proj_st l st__p N ∗
-          (⌜Nat.odd N⌝
-           → ∀ st__t' : amSt odd_AM,
-               ⌜amTrans odd_AM st__t (inl (step_sync N), Some ρ__t)
-                  st__t'⌝ ∗ ⌜cur_odd st__t' (N + 1)⌝
-               → ∃ st__p' : M__p,
-                   ⌜glob_step_odd proj_st lift_role st__p st__p' ρ__t st__t'%nat⌝ ∗
-                   (▷ odd_corr threadG0 proj_st l st__p' (N + 1) ={⊤ ∖ ↑ι,⊤}=∗ True)) ∗
-          (⌜Nat.even N⌝
-           → ∀ (st__t' : amSt odd_AM) (a : oPriv),
-               ⌜amTrans odd_AM st__t (inr a, Some ρ__t) st__t'⌝ ∗
-               ⌜cur_odd st__t' N⌝
-               → ∃ st__p' : M__p,
-                   ⌜glob_step_odd proj_st lift_role st__p st__p' ρ__t st__t'⌝ ∗
-                   (▷ odd_corr threadG0 proj_st l st__p' N ={⊤ ∖ ↑ι,⊤}=∗ True))))%I;
-  odd_prog: val;
-  odd_spec {M__p : FairModel} {LM__p : LiveModel heap_lang M__p} 
-  {Σ : gFunctors} {heapGS0 : heapGS Σ LM__p} {threadG0 : threadG Σ} 
-  (proj_st : M__p → amSt odd_AM) (lift_role: amRole odd_AM → fmrole M__p) 
-  (tid : locale heap_lang) (n : loc) (ρ__t : amRole odd_AM) 
-  (N f : nat) (FUEL: f > 40) (ι : namespace) (FL: ∀ st : M__p, lm_fl LM__p st ≥ 61):
-      {{{ odd_vs proj_st lift_role n ι ρ__t ∗
-        tid ↦M {[lift_role ρ__t := f]} ∗
-        own th_name (◯E N) ∗
-        frag_free_roles_are ∅ }}}
-          odd_prog #n #N@tid
-        {{{ RET #(); tid ↦M ∅ }}};
-
-  ρ__o: amRole odd_AM;
+    ρ__o: amRole odd_AM;
 }.
-
