fairis/heap_lang/examples/even_odd/thread_progs.v
@@ -1,0 +1,155 @@
+From stdpp Require Import decidable.
+From iris.prelude Require Import options.
+From iris.algebra Require Import excl_auth.
+From iris.bi Require Import bi.
+From iris.base_logic.lib Require Import invariants.
+From iris.proofmode Require Import tactics.
+From trillium.prelude Require Export finitary quantifiers sigma classical_instances.
+From trillium.program_logic Require Export weakestpre.
+From trillium.fairness Require Import fairness.
+From trillium.fairness.heap_lang Require Export lang lifting tactics proofmode.
+From trillium.fairness.heap_lang Require Import notation.
+From trillium.fairness.heap_lang.examples.even_odd Require Import action_model utils. 
+
+Close Scope Z. 
+
+
+Class threadG Σ := ThreadG {
+  th_name: gname;
+  th_n_G :> inG Σ (excl_authR natO);
+}.
+
+Class threadPreG Σ := {
+  thread_PreG :> inG Σ (excl_authR natO);
+}.
+
+
+Section ThreadGLemmas.
+  Context `{!threadG Σ}.
+
+  Definition th_at (n: nat) := own th_name (◯E n).
+  Definition auth_th_at (n: nat) := own th_name (●E n).
+  
+  Lemma th_agree γ (N M: nat) :
+    own γ (◯E N) -∗ own γ (●E M) -∗ ⌜ M = N ⌝.
+  Proof.
+    iIntros "HA HB". iCombine "HB HA" as "H".
+    iDestruct (own_valid with "H") as "%Hval".
+    iPureIntro. by apply excl_auth_agree_L.
+  Qed.
+  
+  Lemma th_update γ (N M P: nat) :
+    own γ (●E N) ∗ own γ (◯E M) ==∗ own γ (●E P) ∗ own γ (◯E P).
+  Proof.
+    rewrite -!own_op. iApply own_update. apply excl_auth_update.
+  Qed.
+
+End ThreadGLemmas.
+
+
+Section ProofsGen.  
+  Context `{LM__p: LiveModel heap_lang M__p}.
+  Context `{!heapGS Σ LM__p}.
+  (* Context (d: nat).  *)
+  Context (cond: nat -> bool).
+  Hypothesis (COND_S_NEG: forall n, cond (S n) = negb (cond n)). 
+  
+  Context `{!threadG Σ}.
+  
+  Definition incr_loop : val :=
+    rec: "incr_loop" "l" "n" :=
+      (if: CAS "l" "n" ("n"+ #1)
+       then "incr_loop" "l" ("n" + #2)
+       else "incr_loop" "l" "n").
+  
+  Definition eo_corr l (st: fmstate M__p) (N: nat): iProp Σ :=
+    frag_model_is st ∗ l ↦ #N ∗
+    (* own th_name (●E (if Nat.even (N + d) then N else (N + 1))). *)
+    own th_name (●E (if cond N then N else (N + 1))).
+    
+  Definition eo_vs l ι (ρ: fmrole M__p) tid : iProp Σ :=
+    □ |={⊤, ⊤ ∖ ↑ι}=> ∃ st__p N,
+    (▷ eo_corr l st__p N) ∗
+      (∀ f, tid ↦M {[ ρ := f ]} -∗ frag_model_is st__p -∗ frag_free_roles_are ∅ -∗
+              MU (⊤ ∖ ↑ι) tid (
+                ∃ st__p' f', tid ↦M {[ ρ := f' ]}  ∗ frag_model_is st__p' ∗ frag_free_roles_are ∅ ∗ ⌜ f' > 43 ⌝ ∗
+                                                                                                               (▷ (eo_corr l st__p' (if cond N then N + 1 else N)) ={⊤ ∖ ↑ι, ⊤}=∗ True))).
+  
+  Lemma eo_go_spec (tid: locale heap_lang) n ρ (N: nat) f (Hf: f > 40) ι
+    (FL: forall st, lm_fl LM__p st >= 61):
+    {{{  eo_vs n ι ρ tid ∗
+           has_fuels tid {[ ρ := f ]} ∗ own th_name (◯E N) ∗
+           frag_free_roles_are ∅
+    }}}
+      incr_loop #n #N @ tid
+      {{{ RET #(); has_fuels tid ∅ }}}.
+  Proof using COND_S_NEG.
+    iLöb as "Hg" forall (N f Hf).
+    iIntros (Φ). iIntros "(#VS & Hf & Heven & HFR) Hk".
+                   
+    rewrite /incr_loop.
+    wp_lam.
+    wp_pures. wp_bind (CmpXchg _ _ _). iApply wp_atomic.
+    iPoseProof "VS" as "-#V". iMod "V" as "(%st & %M & (>Hmod & >Hn & >Hauths) & CLOS)".
+
+    (* destruct (Nat.even (M + d)) eqn:Heqn. *)
+    destruct (cond M) eqn:Heqn.
+    - iDestruct (th_agree with "Heven Hauths") as "->".
+      iModIntro.
+      iSpecialize ("CLOS" with "[$] [$] [$]"). 
+      iApply sswp_MU_wp; [done| ].
+      iApply (wp_cmpxchg_suc with "[$]"); try done.  
+      iIntros "!> Hb".
+      iApply (MU_wand with "[-CLOS] [$]"). 
+      iIntros "(%st' & %f' & (Hf& Hmod& HFR & %FUEL' & CLOS))".
+
+      iMod (th_update _ _ _ (N + 2) with "[$]") as "[Hay Heven]".
+      wp_pures.
+      iModIntro. 
+      iMod ("CLOS" with "[Hmod Hay Hb]") as "_". 
+      { replace (Z.of_nat N + 1)%Z with (Z.of_nat (N + 1)) by lia.
+        iFrame.
+        rewrite Nat.add_1_r COND_S_NEG Heqn. simpl.
+        by rewrite Nat.add_succ_r. }
+      iModIntro. simpl.
+
+      pose proof (FL st').
+      do 3 wp_pure _.
+      replace (Z.of_nat N + 2)%Z with (Z.of_nat (N + 2)) by lia.
+      iApply ("Hg" with "[] [Heven Hf HFR] [$]"); last first.
+      { iFrame "∗#". }
+      iPureIntro; lia.
+    - iDestruct (th_agree with "Heven Hauths") as "%Heq". rewrite -> Heq in *.
+      iModIntro.
+      subst.
+
+      iSpecialize ("CLOS" with "[$] [$] [$]"). 
+      iApply sswp_MU_wp; [done| ].
+      iApply (wp_cmpxchg_fail with "[$]"); [| done| ].
+      { assert (M ≠ M + 1) by lia. set_solver. }
+      iIntros "!> Hb".
+      iApply (MU_wand with "[-CLOS] [$]"). 
+      iIntros "(%st' & %f' & (Hf& Hmod& HFR & %FUEL' & CLOS))".
+
+      iMod (th_update _ _ _ (M + 1) with "[$]") as "[Hay Heven]".
+      wp_pures.
+      iModIntro. 
+      iMod ("CLOS" with "[Hmod Hay Hb]") as "_". 
+      { iFrame. by rewrite Heqn. }
+      iModIntro. simpl.
+
+      pose proof (FL st').
+      do 2 wp_pure _.
+      iApply ("Hg" with "[] [Heven Hf HFR] [$]"); last first.
+      { iFrame "∗#". }
+      iPureIntro; lia.
+  Qed.
+    
+End ProofsGen.
+
+
+Definition even_spec `{LM__p: LiveModel heap_lang M__p} `{!heapGS Σ LM__p, !threadG Σ}:=
+    eo_go_spec Nat.even even_succ_negb. 
+
+Definition odd_spec `{LM__p: LiveModel heap_lang M__p} `{!heapGS Σ LM__p, !threadG Σ}:=
+    eo_go_spec Nat.odd odd_succ_negb.
